Main.init

steel/Zeta.Steel.Main.fst
@@ -23,8 +23,155 @@ module SA = Zeta.SeqAux
 
 module Loops = Steel.ST.Loops
 
+assume val create_verifier (tid:tid)
+  : STT V.thread_state_t
+    emp
+    (fun t -> V.thread_state_inv t (M.init_thread_state_model tid))
+
+let init_thread_state
+  (#m:TLM.repr)
+  (mlogs:TLM.t)
+  (i:tid)
+  (_:squash (Map.sel m i == Some Seq.empty))
+  : ST (thread_state mlogs)
+       (TLM.tids_pts_to mlogs half m false)
+       (fun st -> TLM.tids_pts_to mlogs half (Map.upd m i None) false)
+       (requires True)
+       (ensures fun st -> st.tid == i)
+  = let st = create_verifier i in
+    TLM.take_tid mlogs m i;
+    rewrite
+      (TLM.tid_pts_to _ _ _ _ _)
+      (TLM.tid_pts_to mlogs
+                      (M.init_thread_state_model i).M.thread_id
+                      half
+                      (M.init_thread_state_model i).M.processed_entries
+                      false);
+    intro_exists (M.init_thread_state_model i)
+                 (fun tsm -> V.thread_state_inv st tsm
+                            `star`
+                          TLM.tid_pts_to mlogs tsm.M.thread_id half tsm.M.processed_entries false);
+    rewrite
+      (exists_ (fun tsm -> V.thread_state_inv st tsm
+                          `star`
+                        TLM.tid_pts_to mlogs tsm.M.thread_id half tsm.M.processed_entries false))    
+      (thread_inv st mlogs);
+    let lock = Lock.new_lock (thread_inv st mlogs) in
+    return ({tid = i; tsm = st; lock = lock})
+
+let tid_positions_ok_until #l (all_threads:Seq.seq (thread_state l)) (i:nat)
+  : prop
+  = forall (j:SA.seq_index all_threads).
+      j < i ==> (let sj = Seq.index all_threads j in
+                 U16.v sj.tid == j)
+
+let rec init_all_threads_state
+  (#m:TLM.repr)
+  (#mlogs:TLM.t)
+  (all_threads:all_threads_t mlogs)
+  (i:U16.t{U16.v i <= U32.v n_threads})
+  : ST unit
+       (TLM.tids_pts_to mlogs half m false
+          `star`
+        exists_ (fun s -> A.pts_to all_threads full_perm s
+                         `star`
+                       pure (tid_positions_ok_until s (U16.v i))))
+                   
+       (fun _ -> exists_ (fun s -> A.pts_to all_threads full_perm s
+                               `star`
+                             pure (tid_positions_ok_until s (Seq.length s))))
+       (requires forall (j:tid). U16.v i <= U16.v j ==> Map.sel m j == Some Seq.empty)
+       (ensures fun _ -> True)
+  = let s = elim_exists () in
+    A.pts_to_length all_threads s;
+    elim_pure (tid_positions_ok_until s (U16.v i));
+    let b = FStar.Int.Cast.uint16_to_uint32 i = n_threads in
+    if b returns STT _ _ (fun _ -> exists_ (fun s -> A.pts_to all_threads full_perm s
+                                  `star`
+                                pure (tid_positions_ok_until s (Seq.length s))))
+
+    then begin
+      intro_pure (tid_positions_ok_until s (Seq.length s));
+      drop (TLM.tids_pts_to _ _ _ _);
+      intro_exists
+        (Ghost.reveal s)
+        (fun s -> A.pts_to all_threads full_perm s
+                 `star`
+               pure (tid_positions_ok_until s (Seq.length s)));
+      return ()
+    end
+    else begin
+      let st = init_thread_state mlogs i () in
+      A.write all_threads (FStar.Int.Cast.uint16_to_uint32 i) st;
+      rewrite
+        (A.pts_to all_threads full_perm (Seq.upd s (U32.v (FStar.Int.Cast.uint16_to_uint32 i)) st))
+        (A.pts_to all_threads full_perm (Seq.upd s (U16.v i) st));
+      intro_pure (tid_positions_ok_until (Seq.upd s (U16.v i) st) (U16.v (U16.add i 1us)));
+      intro_exists
+        (Seq.upd s (U16.v i) st)
+        (fun s -> A.pts_to all_threads full_perm s
+                 `star`
+               pure (tid_positions_ok_until s (U16.v (U16.add i 1us))));
+      init_all_threads_state #(Map.upd m i None) #mlogs all_threads (U16.add i 1us)
+    end
+
+let init_aux (#opened:_)
+  (aeh:AEH.aggregate_epoch_hashes)
+  (all_threads:all_threads_t aeh.mlogs)
+  (t:top_level_state)
+  (s:Ghost.erased (Seq.seq (thread_state aeh.mlogs)))
+  : STGhost unit opened
+      (pure (tid_positions_ok s)
+         `star`
+       A.pts_to all_threads full_perm s
+         `star`
+       TLM.tids_pts_to aeh.mlogs half (Map.const (Some Seq.empty)) false)
+      (fun _ -> core_inv t
+               `star`
+             TLM.tids_pts_to t.aeh.mlogs half (Map.const (Some Seq.empty)) false)
+      (requires t.aeh == aeh /\ t.all_threads == all_threads)
+      (ensures fun _ -> True)
+  = rewrite (A.pts_to all_threads full_perm s)
+            (A.pts_to t.all_threads full_perm s);
+    rewrite (TLM.tids_pts_to aeh.mlogs half (Map.const (Some Seq.empty)) false)
+            (TLM.tids_pts_to t.aeh.mlogs half (Map.const (Some Seq.empty)) false);
+    rewrite (pure (tid_positions_ok s))
+            (pure (tid_positions_ok #(t.aeh.mlogs) s));
+    intro_exists
+      (Ghost.reveal s)
+      (fun s -> A.pts_to t.all_threads full_perm s
+               `star`
+             pure (tid_positions_ok s));
+    intro_exists
+      full_perm
+      (fun perm -> exists_ (fun s -> A.pts_to t.all_threads perm s
+                                 `star`
+                               pure (tid_positions_ok s)));
+    rewrite (exists_ _) (core_inv t)
+
 let init () =
   let aeh = AEH.create () in
-  //TLM.tids_pts_to aeh.mlogs full_perm (Map.const (Some Seq.empty)) false
-  
-  admit___ ()
+  TLM.share_tids_pts_to aeh.mlogs (Map.const (Some Seq.empty));
+  let st0 = init_thread_state aeh.mlogs 0us () in
+  let all_threads = A.alloc st0 n_threads in
+  intro_pure (tid_positions_ok_until (Seq.create (U32.v n_threads) st0) 1);
+  intro_exists
+    (Seq.create (U32.v n_threads) st0)
+    (fun s -> A.pts_to all_threads full_perm s
+             `star`
+           pure (tid_positions_ok_until s 1));
+  init_all_threads_state
+    #(Map.upd (Map.const (Some Seq.empty)) 0us None)
+    #aeh.mlogs
+    all_threads
+    1us;
+
+  let s = elim_exists () in
+  A.pts_to_length all_threads s;
+  elim_pure (tid_positions_ok_until s (Seq.length s));
+
+  intro_pure (tid_positions_ok s);
+
+  let r = ({ aeh = aeh; all_threads = all_threads }) in
+  init_aux aeh all_threads r s;
+  return r
